src/Lean/Meta/Tactic/Grind/EMatch.lean
@@ -104,7 +104,7 @@ private def matchArg? (c : Choice) (pArg : Expr) (eArg : Expr) : OptionT GoalM C
   else if pArg.isBVar then
     assign? c pArg.bvarIdx! eArg
   else if let some pArg := groundPattern? pArg then
-    guard (← isEqv pArg eArg)
+    guard (← isEqv pArg eArg <||> withReducible (isDefEq pArg eArg))
     return c
   else if let some (pArg, k) := isOffsetPattern? pArg then
     assert! Option.isNone <| isOffsetPattern? pArg
