tests/lean/run/grind_constProp.lean
@@ -201,13 +201,14 @@ def evalExpr (e : Expr) : EvalM Val := do
   | una op arg => op.simplify arg.simplify
   | e => e
 
+@[grind] theorem BinaryOp.simplify_eval (op : BinOp) : (op.simplify a b).eval σ = (Expr.bin a op b).eval σ := by
+  grind [BinOp.simplify.eq_def]
+
+@[grind] theorem UnaryOp.simplify_eval (op : UnaryOp) : (op.simplify a).eval σ = (Expr.una op a).eval σ := by
+  grind [UnaryOp.simplify.eq_def]
+
 @[simp, grind =] theorem Expr.eval_simplify (e : Expr) : e.simplify.eval σ = e.eval σ := by
-  induction e <;> try grind [BinOp.simplify.eq_def, UnaryOp.simplify.eq_def]
-  next op arg ih_arg =>
-    simp only [simplify, UnaryOp.simplify, eval, ← ih_arg, UnaryOp.eval]
-    split
-    · grind
-    · simp only [eval, UnaryOp.eval] -- TODO: `grind` failes here
+  induction e, σ using Expr.simplify.induct <;> grind
 
 @[simp, grind =] def Stmt.simplify : Stmt → Stmt
   | skip => skip
@@ -306,13 +307,12 @@ theorem State.cons_le_of_eq (h₁ : σ' ≼ σ) (h₂ : σ.find? x = some v) : (
 @[grind] theorem State.join_le_right_of (h : σ₁ ≼ σ₂) (σ₃ : State) : σ₃.join σ₁ ≼ σ₂ := by
   grind
 
+@[grind] theorem not_cons_le_nil : ¬ (x, v) :: σ ≼ [] := by
+  -- Remark: `grind` fails here because it is not capable of "guessing" that we need to instantiate the hypothesis with `x`
+  intro h; have h := @h x; simp at h
+
 theorem State.eq_bot (h : σ ≼ ⊥) : σ = ⊥ := by
-  match σ with
-  | [] => grind
-  | (y, v) :: σ =>
-    -- TODO: can we avoid this hint?
-    have : State.find? ((y, v) :: σ) y = some v := by grind
-    grind
+  grind [cases Prod, cases List]
 
 theorem State.erase_le_of_le_cons (h : σ' ≼ (x, v) :: σ) : σ'.erase x ≼ σ := by
   grind
